%        File: newfile.tex
%     Created: Sun Sep 24 08:00 PM 2017 AEST
% Last Change: Sun Sep 24 08:00 PM 2017 AEST
%
\documentclass[a4paper]{article}

\usepackage[sumlimits,]{amsmath}
\usepackage{amssymb}
\usepackage{parskip}

\begin{document}
Conjecture: Prove that for any natural number $n$, $2 + 2^2 + 2^3 + \dots + 2^n = 2^{n+1} - 2$

Let $A(n): 2 + 2^2 + 2^3 + \dots + 2^n = 2^{n+1} - 2$

Proof by induction,

$A(1): 2 = 2^2 - 2$

Assuming $A(n)$ is true then,
\begin{align*}
  A(n+1): 2 + 2^2 + 2^3 + \dots + 2^{n+1} &= 2^{n+1} - 2 + 2^{n+1} && \text{[Induction hypothesis]} \\
  &= 2(2^{n+1}) - 2 && \text{[Algebra]} \\
  &= 2^{n+2} - 2 && \text{[Algebra]}
\end{align*}

Therefore, the conjecture is true.

\end{document}
